introduce extra status BST_AssertionViolated
Before, the status was BST_failed, if an assertion got violated. While
BST_AssertionViolated is still a failure for e.g. Hoare-triples, it
allows to reason about programs more fine-grained. We can now
distinguish that a program fails, because an assertion is violated
(which is kind of "expected" sometimes (otherwise you could remove the
assertions) or whether the program fails because it is not well-formed
in some sense (which should be avoided). In particular this allows us to
show that the programs produced by the program lifter only fail, if an
assertion is violated.

src/core/bir_programScript.sml
@@ -56,6 +56,7 @@ val _ = Datatype `bir_status_t =
     BST_Running                  (* BIR program is still running *)
   | BST_Failed                   (* BIR program execution failed *)
   | BST_AssumptionViolated       (* BIR program execution aborted, because assumption was violated *)
+  | BST_AssertionViolated       (* BIR program execution failed, because assertion was violated *)
   | BST_Halted bir_val_t        (* Halt called *)
   | BST_JumpOutside bir_label_t (* Jump to unknown label *)`;
 
@@ -187,7 +188,7 @@ val bir_exec_stmt_assign_def = Define `bir_exec_stmt_assign v ex (st : bir_state
 val bir_exec_stmt_assert_def = Define `bir_exec_stmt_assert ex (st : bir_state_t) =
   case (bir_dest_bool_val (bir_eval_exp ex st.bst_environ)) of
     | SOME T => st
-    | SOME F => bir_state_set_failed st
+    | SOME F => (st with bst_status := BST_AssertionViolated)
     | NONE => bir_state_set_failed st`
 
 val bir_exec_stmt_assume_def = Define `bir_exec_stmt_assume ex (st : bir_state_t) =
